\documentclass{article}
\input{503macros.tex}

\begin{document}
\begin{center}
  {\LARGE CSC 503 Homework Assignment 5}\\[1pc]
  Out: September 25, 2018 \\
  Due: October 3, 2018 \\
  \unityid{MISSING}
\end{center}

If using the Fitch macros to typeset proofs in first order logic, one
introduces a dummy variable $x$ by means of the command
\verb+\open[x]+. 

\begin{enumerate}
\item[1.] \textbf{[20 points]} Using only the basic natural deduction
  rules, prove  the sequent
  \begin{displaymath}
    \forall x \forall y (\neg R(y) \implies S(x))
    \turn
    (\exists y \neg R(y)) \implies (\forall x S(x)).
\end{displaymath}
\end{enumerate}

\begin{enumerate}
\item[2.] \textbf{[20 points]} Using only the basic natural deduction
  rules, prove  the sequent
  \begin{displaymath}
    \forall x (P(x) \implies \neg R(x))
    \turn
    \neg( \exists x ( P(x) \land R(x))).
  \end{displaymath}
\end{enumerate}

\begin{enumerate}
\item[3.] \textbf{[10 points]} Using only the basic natural deduction
  rules, prove  the sequent
  \begin{displaymath}
    \forall x\ P(a,f(a),x),
    \forall z \forall x \forall y\ (P(x,y,z) \implies P(f(x),y,f(f(z)))) 
    \turn
    P(f(a),f(a),f(f(f(a)))).
  \end{displaymath}
\end{enumerate}

\begin{enumerate}
\item[4.] \textbf{[20 points]} Using only the basic natural deduction
  rules, prove  the sequent
  \begin{displaymath}
    \exists x \forall y \forall z P(x,y,z)
    \turn
    \forall z \forall y \exists x P(x,y,z).
\end{displaymath}
\end{enumerate}

\begin{enumerate}
\item[5.] \textbf{[10 points]} Using only the basic natural deduction
  rules, prove the sequent
  \begin{displaymath}
    \forall x \forall y\ [S(x,y) \implies \neg S(y,x)]
    \turn
    \forall x\ \neg S(x,x)
  \end{displaymath}
\end{enumerate}

\begin{enumerate}
\item[6.] \textbf{[20 points]} Using only the basic natural deduction
  rules, prove the sequent
  \begin{displaymath}
    \forall x \forall y \forall z [(S(x,y) \land S(y,z)) \implies
    S(x,z)],
    \forall x \neg S(x,x)
    \turn
    \forall x \forall y [S(x,y) \implies \neg S(y,x)]
  \end{displaymath}
\end{enumerate}

\end{document}

